doc/coq/simple/Concrete.v
@@ -39,7 +39,7 @@ Inductive EvalR `{time T} (C : @dy_ctx T) (st : @state T)
                          (EVal (Closure x e C_lam)) st_lam)
              (ARG : EvalR C st_lam e2
                           (EVal arg) (ST mem t))
-             (BODY : EvalR (C_lam [|dy_c_lam x t ([||])|])
+             (BODY : EvalR (C_lam [|dy_binde x t ([||])|])
                            (ST (t !-> arg ; mem) (tick C (ST mem t) x arg))
                            e (EVal v) st_v)
     : EvalR C st (e_app e1 e2) (EVal v) st_v
@@ -54,14 +54,14 @@ Inductive EvalR `{time T} (C : @dy_ctx T) (st : @state T)
   | Eval_lete x e v mem t
               m C_m st_m
                (EVALe : EvalR C st e (EVal v) (ST mem t))
-               (EVALm : EvalR (C [|dy_c_lete x t ([||])|])
+               (EVALm : EvalR (C [|dy_binde x t ([||])|])
                         (ST (t !-> v ; mem) (tick C (ST mem t) x v))
                         m (MVal C_m) st_m)
     : EvalR C st (m_lete x e m) (MVal C_m) st_m
   | Eval_letm M m' C' st'
               m'' C'' st''
               (EVALm' : EvalR C st m' (MVal C') st')
-              (EVALm'' : EvalR (C [|dy_c_letm M C' ([||])|]) st'
+              (EVALm'' : EvalR (C [|dy_bindm M C' ([||])|]) st'
                          m'' (MVal C'') st'')
     : EvalR C st (m_letm M m' m'') (MVal C'') st''
 .
@@ -104,7 +104,7 @@ Fixpoint eval `{time T} (C : @dy_ctx T) (st : @state T)
       | Resolved (EVal (Closure x e' C_lam)) st_lam reached' =>
         match eval C st_lam e2 reached' FUEL' with
         | Resolved (EVal arg) (ST mem t) reached'' =>
-          match eval (C_lam [| dy_c_lam x t ([||]) |]) 
+          match eval (C_lam [| dy_binde x t ([||]) |]) 
                      (ST (t !-> arg ; mem) (tick C (ST mem t) x arg)) 
                      e' reached'' FUEL' with
           | Resolved (EVal v) st' reached''' => Resolved (EVal v) st' reached'''
@@ -136,7 +136,7 @@ Fixpoint eval `{time T} (C : @dy_ctx T) (st : @state T)
     | m_lete x e m =>
       match eval C st e reached FUEL' with
       | Resolved (EVal v) (ST mem t) reached' =>
-        match eval (C[| dy_c_lete x t ([||]) |]) 
+        match eval (C[| dy_binde x t ([||]) |]) 
                    (ST (t !-> v ; mem) (tick C (ST mem t) x v)) 
                    m reached' FUEL' with
         | Resolved (MVal C') st' reached'' => Resolved (MVal C') st' reached''
@@ -149,7 +149,7 @@ Fixpoint eval `{time T} (C : @dy_ctx T) (st : @state T)
     | m_letm M m1 m2 =>
       match eval C st m1 reached FUEL' with
       | Resolved (MVal C') st' reached' =>
-        match eval (C[| dy_c_letm M C' ([||]) |])
+        match eval (C[| dy_bindm M C' ([||]) |])
                    st' m2 reached' FUEL' with
         | Resolved (MVal C'') st'' reached'' => Resolved (MVal C'') st'' reached''
         | Resolved _ _ reached'' => Error reached''
@@ -179,7 +179,7 @@ Proof.
       destruct v2 as [ | | v2 st2]; inversion H;
       clear H3. destruct v2 as [v2 | ]; inversion H.
       clear H3. destruct st2 as [mem2 t2].
-      remember (eval (C_lam [|dy_c_lam x t2 ([||])|]) 
+      remember (eval (C_lam [|dy_binde x t2 ([||])|]) 
                      (ST (t2 !-> v2; mem2) (tick C (ST mem2 t2) x v2))
                       v1 reached0 FUEL) as v3.
       destruct v3 as [ | | v3 st3]; inversion H.
@@ -189,7 +189,7 @@ Proof.
       apply IHFUEL; eauto. nia.
       assert (eval C st1 e2 reached m = Resolved (EVal v2) (ST mem2 t2) reached0) as RR2.
       apply IHFUEL; eauto. nia.
-      assert (eval (C_lam [|dy_c_lam x t2 ([||])|])
+      assert (eval (C_lam [|dy_binde x t2 ([||])|])
                    (ST (t2 !-> v2; mem2) (tick C (ST mem2 t2) x v2)) v1 reached0 m = 
               Resolved (EVal v3) st' l') as RR3.
       apply IHFUEL; eauto. nia.
@@ -212,7 +212,7 @@ Proof.
       destruct v1 as [ | | v1 st1]; inversion H.
       clear H3. destruct v1 as [v1 | ]; inversion H.
       clear H3. destruct st1 as [mem1 t1].
-      remember (eval (C [|dy_c_lete x t1 ([||])|]) 
+      remember (eval (C [|dy_binde x t1 ([||])|]) 
                      (ST (t1 !-> v1; mem1) (tick C (ST mem1 t1) x v1))
                       e2 reached FUEL) as v2.
       destruct v2 as [ | | v2 st2]; inversion H.
@@ -220,7 +220,7 @@ Proof.
       subst.
       assert (eval C st e1 (Config C st (m_lete x e1 e2) :: l) m = Resolved (EVal v1) (ST mem1 t1) reached) as RR1.
       apply IHFUEL; eauto. nia.
-      assert (eval (C [|dy_c_lete x t1 ([||])|]) 
+      assert (eval (C [|dy_binde x t1 ([||])|]) 
                    (ST (t1 !-> v1; mem1) (tick C (ST mem1 t1) x v1))
                    e2 reached m = Resolved (MVal mv) st' l') as RR2.
       apply IHFUEL; eauto. nia.
@@ -229,14 +229,14 @@ Proof.
       destruct v1 as [ | | v1 st1]; inversion H.
       clear H3. destruct v1 as [v1 | ]; inversion H.
       clear H3.
-      remember (eval (C [|dy_c_letm M mv ([||])|]) st1
+      remember (eval (C [|dy_bindm M mv ([||])|]) st1
                       e2 reached FUEL) as v2.
       destruct v2 as [ | | v2 st2]; inversion H.
       clear H3. destruct v2 as [v2 | ]; inversion H.
       subst.
       assert (eval C st e1 (Config C st (m_letm M e1 e2) :: l) m = Resolved (MVal mv) st1 reached) as RR1.
       apply IHFUEL; eauto. nia.
-      assert (eval (C [|dy_c_letm M mv ([||])|]) st1
+      assert (eval (C [|dy_bindm M mv ([||])|]) st1
                    e2 reached m = Resolved (MVal mv0) st' l') as RR2.
       apply IHFUEL; eauto. nia.
       simpl. rewrite RR1. rewrite RR2. eauto.
@@ -258,7 +258,7 @@ Proof.
     destruct (IHR2 reached) as [FUEL'' EQ'']. clear IHR2.
     destruct (eval C st_lam e2 reached FUEL'') eqn:EVAL2; try (inversion EQ''; fail).
     destruct (IHR3 reached0) as [FUEL''' EQ''']. clear IHR3.
-    destruct (eval (C_lam [|dy_c_lam x t ([||])|])
+    destruct (eval (C_lam [|dy_binde x t ([||])|])
                    (ST (t !-> arg; mem) (tick C (ST mem t) x arg)) e reached0
                    FUEL''') eqn:EVAL3; try (inversion EQ'''; fail).
     exists (S (Nat.max FUEL' (Nat.max FUEL'' FUEL'''))).
@@ -274,7 +274,7 @@ Proof.
             = Resolved (EVal arg) (ST mem t) reached0) as RR.
     apply relax_fuel with (FUEL := FUEL''). nia. eauto.
     rewrite RR; clear RR.
-    assert (eval (C_lam [|dy_c_lam x t ([||])|]) 
+    assert (eval (C_lam [|dy_binde x t ([||])|]) 
                  (ST (t !-> arg; mem) (tick C (ST mem t) x arg)) e reached0
                  (Nat.max FUEL' (Nat.max FUEL'' FUEL'''))
             = Resolved (EVal v) st_v reached1) as RR.
@@ -301,7 +301,7 @@ Proof.
   - destruct (IHR1 (Config C st (m_lete x e m) :: l)) as [FUEL' EQ']. clear IHR1.
     destruct (eval C st e (Config C st (m_lete x e m) :: l) FUEL') eqn:EVAL1; try (inversion EQ'; fail).
     destruct (IHR2 reached) as [FUEL'' EQ'']. clear IHR2.
-    destruct (eval (C [|dy_c_lete x t ([||])|])
+    destruct (eval (C [|dy_binde x t ([||])|])
                    (ST (t !-> v; mem) (tick C (ST mem t) x v)) m reached
                    FUEL'') eqn:EVAL2; try (inversion EQ''; fail).
     exists (S (Nat.max FUEL' FUEL'')).
@@ -312,7 +312,7 @@ Proof.
             = Resolved (EVal v) (ST mem t) reached) as RR.
     apply relax_fuel with (FUEL := FUEL'). nia. eauto.
     rewrite RR; clear RR.
-    assert (eval (C [|dy_c_lete x t ([||])|]) 
+    assert (eval (C [|dy_binde x t ([||])|]) 
                  (ST (t !-> v; mem) (tick C (ST mem t) x v)) m reached
                  (Nat.max FUEL' FUEL'')
             = Resolved (MVal C_m) st_m reached0) as RR.
@@ -321,7 +321,7 @@ Proof.
   - destruct (IHR1 (Config C st (m_letm M m' m'') :: l)) as [FUEL' EQ']. clear IHR1.
     destruct (eval C st m' (Config C st (m_letm M m' m'') :: l) FUEL') eqn:EVAL1; try (inversion EQ'; fail).
     destruct (IHR2 reached) as [FUEL'' EQ'']. clear IHR2.
-    destruct (eval (C [|dy_c_letm M C' ([||])|]) st' m'' reached FUEL'') eqn:EVAL2; try (inversion EQ''; fail).
+    destruct (eval (C [|dy_bindm M C' ([||])|]) st' m'' reached FUEL'') eqn:EVAL2; try (inversion EQ''; fail).
     exists (S (Nat.max FUEL' FUEL'')).
     simpl.
     destruct EQ' as [RR RR']. rewrite <- RR in *. rewrite <- RR' in *. clear RR RR'.
@@ -330,7 +330,7 @@ Proof.
             = Resolved (MVal C') st' reached) as RR.
     apply relax_fuel with (FUEL := FUEL'). nia. eauto.
     rewrite RR; clear RR.
-    assert (eval (C [|dy_c_letm M C' ([||])|]) st' m'' reached (Nat.max FUEL' FUEL'')
+    assert (eval (C [|dy_bindm M C' ([||])|]) st' m'' reached (Nat.max FUEL' FUEL'')
             = Resolved (MVal C'') st'' reached0) as RR.
     apply relax_fuel with (FUEL := FUEL''). nia. eauto.
     rewrite RR; clear RR. eauto.
@@ -359,7 +359,7 @@ Proof.
     destruct v2 as [ | | v2 st2]; try inversion R.
     destruct v2 as [v2 | ]; try inversion R.
     destruct st2 as [mem2 t2].
-    remember (eval (C_lam [|dy_c_lam x t2 ([||])|])
+    remember (eval (C_lam [|dy_binde x t2 ([||])|])
                    (ST (t2 !-> v2; mem2) (tick C (ST mem2 t2) x v2)) 
                    v1 reached0 FUEL) as v3.
     destruct v3 as [ | | v3 st3]; try inversion R.
@@ -369,7 +369,7 @@ Proof.
     eapply IHFUEL; rewrite <- Heqv1; eauto.
     assert (EvalR C st1 e2 (EVal v2) (ST mem2 t2)) as RR2.
     eapply IHFUEL; rewrite <- Heqv2; eauto.
-    assert (EvalR (C_lam [|dy_c_lam x t2 ([||])|])
+    assert (EvalR (C_lam [|dy_binde x t2 ([||])|])
                   (ST (t2 !-> v2; mem2) (tick C (ST mem2 t2) x v2)) v1
             (EVal v3) st3) as RR3. 
     eapply IHFUEL; rewrite <- Heqv3; eauto. eauto.
@@ -390,14 +390,14 @@ Proof.
     destruct v1 as [ | | v1 st1]; try inversion R.
     destruct v1 as [v1 | ]; try inversion R.
     destruct st1 as [mem1 t1].
-    remember (eval (C [|dy_c_lete x t1 ([||])|])
+    remember (eval (C [|dy_binde x t1 ([||])|])
                    (ST (t1 !-> v1; mem1) (tick C (ST mem1 t1) x v1)) 
                    e2 reached FUEL) as v2.
     destruct v2 as [ | | v2 st2]; try inversion R.
     destruct v2 as [v2 | ]; inversion R.
     assert (EvalR C st e1 (EVal v1) (ST mem1 t1)).
     eapply IHFUEL; rewrite <- Heqv1; eauto.
-    assert (EvalR (C [|dy_c_lete x t1 ([||])|])
+    assert (EvalR (C [|dy_binde x t1 ([||])|])
                   (ST (t1 !-> v1; mem1) (tick C (ST mem1 t1) x v1)) e2
             (MVal mv) st2).
     eapply IHFUEL; rewrite <- Heqv2; eauto.
@@ -405,12 +405,12 @@ Proof.
   - remember (eval C st e1 (Config C st (m_letm M e1 e2) :: l) FUEL) as v1.
     destruct v1 as [ | | v1 st1]; try inversion R.
     destruct v1 as [v1 | ]; try inversion R.
-    remember (eval (C [|dy_c_letm M mv ([||])|]) st1 e2 reached FUEL) as v2.
+    remember (eval (C [|dy_bindm M mv ([||])|]) st1 e2 reached FUEL) as v2.
     destruct v2 as [ | | v2 st2]; try inversion R.
     destruct v2 as [v2 | ]; inversion R.
     assert (EvalR C st e1 (MVal mv) st1).
     eapply IHFUEL; rewrite <- Heqv1; eauto.
-    assert (EvalR (C [|dy_c_letm M mv ([||])|]) st1 e2 (MVal mv0) st2).
+    assert (EvalR (C [|dy_bindm M mv ([||])|]) st1 e2 (MVal mv0) st2).
     eapply IHFUEL; rewrite <- Heqv2; eauto.
     subst. eauto.
 Qed.
@@ -447,7 +447,7 @@ Inductive one_reach `{time T} (C : dy_ctx) (st : state)
                 (ARG : EvalR C st_lam e2
                              (EVal arg) (ST mem t))
     : one_reach C st (e_app e1 e2)
-                (C_lam[|dy_c_lam x t ([||])|]) 
+                (C_lam[|dy_binde x t ([||])|]) 
                 (ST (t !-> arg ; mem) (tick C (ST mem t) x arg)) e
   | one_linkl m e
     : one_reach C st (e_link m e)
@@ -462,7 +462,7 @@ Inductive one_reach `{time T} (C : dy_ctx) (st : state)
   | one_leter x e m v mem t
               (EVALx : EvalR C st e (EVal v) (ST mem t))
     : one_reach C st (m_lete x e m)
-                (C[|dy_c_lete x t ([||])|])
+                (C[|dy_binde x t ([||])|])
                 (ST (t !-> v ; mem) (tick C (ST mem t) x v)) m
   | one_letml M m1 m2
     : one_reach C st (m_letm M m1 m2)
@@ -470,7 +470,7 @@ Inductive one_reach `{time T} (C : dy_ctx) (st : state)
   | one_letmr M m1 m2 C_M st_M
               (EVALM : EvalR C st m1 (MVal C_M) st_M)
     : one_reach C st (m_letm M m1 m2)
-                (C[|dy_c_letm M C_M ([||])|]) st_M m2
+                (C[|dy_bindm M C_M ([||])|]) st_M m2
 .
 
 Inductive multi_reach `{time T} (C : dy_ctx) (st : state)
@@ -506,7 +506,7 @@ Inductive ReachR `{time T} (C : @dy_ctx T) (st : @state T)
                             (EVal (Closure x e C_lam)) st_lam)
                 (ARG : EvalR C st_lam e2
                              (EVal arg) (ST mem t))
-                (REACHb : ReachR (C_lam[|dy_c_lam x t ([||])|]) 
+                (REACHb : ReachR (C_lam[|dy_binde x t ([||])|]) 
                                  (ST (t !-> arg ; mem) (tick C (ST mem t) x arg)) e
                                  C' st' e')
     : ReachR C st (e_app e1 e2)
@@ -530,7 +530,7 @@ Inductive ReachR `{time T} (C : @dy_ctx T) (st : @state T)
   | r_lete_m x e m v mem t
              C' st' e'
              (EVALx : EvalR C st e (EVal v) (ST mem t))
-             (REACHm : ReachR (C[|dy_c_lete x t ([||])|])
+             (REACHm : ReachR (C[|dy_binde x t ([||])|])
                               (ST (t !-> v ; mem) (tick C (ST mem t) x v)) m
                               C' st' e')
     : ReachR C st (m_lete x e m)
@@ -543,7 +543,7 @@ Inductive ReachR `{time T} (C : @dy_ctx T) (st : @state T)
   | r_letm_m2 M m1 m2 C_M st_M
               C' st' e'
               (EVALM : EvalR C st m1 (MVal C_M) st_M)
-              (REACHm : ReachR (C[|dy_c_letm M C_M ([||])|]) st_M m2
+              (REACHm : ReachR (C[|dy_bindm M C_M ([||])|]) st_M m2
                                C' st' e')
     : ReachR C st (m_letm M m1 m2)
              C' st' e'
@@ -624,9 +624,9 @@ Proof.
       destruct (eval C st0 e2 reached FUEL); eauto.
       destruct v; eauto. destruct st1.
       assert (In (Config C st (e_app e1 e2)) reached0); eauto. clear IH IH'.
-      specialize (IHFUEL (C' [|dy_c_lam x t ([||])|]) (ST (t !-> ev; mem) (tick C (ST mem t) x ev)) e reached0) as IH.
+      specialize (IHFUEL (C' [|dy_binde x t ([||])|]) (ST (t !-> ev; mem) (tick C (ST mem t) x ev)) e reached0) as IH.
       destruct IH as [IH IH'].
-      destruct (eval (C' [|dy_c_lam x t ([||])|])
+      destruct (eval (C' [|dy_binde x t ([||])|])
                 (ST (t !-> ev; mem) (tick C (ST mem t) x ev)) e reached0
                 FUEL); eauto.
       destruct v; eauto.
@@ -645,9 +645,9 @@ Proof.
       destruct (eval C st e1 (Config C st (m_lete x e1 e2) :: l) FUEL);
       assert (In (Config C st (m_lete x e1 e2)) reached); try apply IH'; simpl; eauto.
       destruct v; simpl; eauto. destruct st0. clear IH IH'.
-      specialize (IHFUEL (C [|dy_c_lete x t ([||])|]) (ST (t !-> ev; mem) (tick C (ST mem t) x ev)) e2 reached) as IH.
+      specialize (IHFUEL (C [|dy_binde x t ([||])|]) (ST (t !-> ev; mem) (tick C (ST mem t) x ev)) e2 reached) as IH.
       destruct IH as [IH IH'].
-      destruct (eval (C [|dy_c_lete x t ([||])|])
+      destruct (eval (C [|dy_binde x t ([||])|])
                      (ST (t !-> ev; mem) (tick C (ST mem t) x ev)) e2 reached
                      FUEL); eauto.
       destruct v; eauto.
@@ -656,9 +656,9 @@ Proof.
       destruct (eval C st e1 (Config C st (m_letm M e1 e2) :: l) FUEL);
       assert (In (Config C st (m_letm M e1 e2)) reached); try apply IH'; simpl; eauto.
       destruct v; simpl; eauto. clear IH IH'.
-      specialize (IHFUEL (C [|dy_c_letm M mv ([||])|]) st0 e2 reached) as IH.
+      specialize (IHFUEL (C [|dy_bindm M mv ([||])|]) st0 e2 reached) as IH.
       destruct IH as [IH IH'].
-      destruct (eval (C [|dy_c_letm M mv ([||])|]) st0 e2 reached FUEL); eauto.
+      destruct (eval (C [|dy_bindm M mv ([||])|]) st0 e2 reached FUEL); eauto.
       destruct v; eauto.
   - intros. destruct e; simpl; eauto.
     + destruct (addr_x C x); simpl; eauto. destruct st. destruct (mem t); simpl; eauto.
@@ -673,9 +673,9 @@ Proof.
       destruct (eval C st0 e2 reached FUEL); eauto.
       destruct v; eauto. destruct st1.
       assert (In cf reached0); simpl in *; eauto. clear IH IH'.
-      specialize (IHFUEL (C' [|dy_c_lam x t ([||])|]) (ST (t !-> ev; mem) (tick C (ST mem t) x ev)) e reached0) as IH.
+      specialize (IHFUEL (C' [|dy_binde x t ([||])|]) (ST (t !-> ev; mem) (tick C (ST mem t) x ev)) e reached0) as IH.
       destruct IH as [IH IH'].
-      destruct (eval (C' [|dy_c_lam x t ([||])|])
+      destruct (eval (C' [|dy_binde x t ([||])|])
                 (ST (t !-> ev; mem) (tick C (ST mem t) x ev)) e reached0
                 FUEL); eauto.
       destruct v; eauto.
@@ -693,9 +693,9 @@ Proof.
       destruct (eval C st e1 (Config C st (m_lete x e1 e2) :: l) FUEL);
       assert (In cf reached); try apply IH'; simpl; eauto.
       destruct v; simpl; eauto. destruct st0. clear IH IH'.
-      specialize (IHFUEL (C [|dy_c_lete x t ([||])|]) (ST (t !-> ev; mem) (tick C (ST mem t) x ev)) e2 reached) as IH.
+      specialize (IHFUEL (C [|dy_binde x t ([||])|]) (ST (t !-> ev; mem) (tick C (ST mem t) x ev)) e2 reached) as IH.
       destruct IH as [IH IH'].
-      destruct (eval (C [|dy_c_lete x t ([||])|])
+      destruct (eval (C [|dy_binde x t ([||])|])
                      (ST (t !-> ev; mem) (tick C (ST mem t) x ev)) e2 reached
                      FUEL); eauto.
       destruct v; eauto.
@@ -704,9 +704,9 @@ Proof.
       destruct (eval C st e1 (Config C st (m_letm M e1 e2) :: l) FUEL);
       assert (In cf reached); try apply IH'; simpl; eauto.
       destruct v; simpl; eauto. clear IH IH'.
-      specialize (IHFUEL (C [|dy_c_letm M mv ([||])|]) st0 e2 reached) as IH.
+      specialize (IHFUEL (C [|dy_bindm M mv ([||])|]) st0 e2 reached) as IH.
       destruct IH as [IH IH'].
-      destruct (eval (C [|dy_c_letm M mv ([||])|]) st0 e2 reached FUEL); eauto.
+      destruct (eval (C [|dy_bindm M mv ([||])|]) st0 e2 reached FUEL); eauto.
       destruct v; eauto.
 Qed.
 
@@ -730,11 +730,11 @@ Proof.
         destruct v; eauto; destruct ev;
         destruct (eval C st0 e2 reached0 m); eauto;
         destruct v; eauto; destruct st1;
-        assert (In cf (extract_reached (eval (C0 [|dy_c_lam x t ([||])|])
+        assert (In cf (extract_reached (eval (C0 [|dy_binde x t ([||])|])
                                              (ST (t !-> ev; mem) (tick C (ST mem t) x ev)) e
                                              reached1 m))) as HINT'';
         try (apply reach_myself; apply HINT');
-        destruct (eval (C0 [|dy_c_lam x t ([||])|])
+        destruct (eval (C0 [|dy_binde x t ([||])|])
                        (ST (t !-> ev; mem) (tick C (ST mem t) x ev)) e
                        reached1 m); eauto; destruct v; eauto; fail);
       pose proof (relax_fuel C st e1 (Config C st (e_app e1 e2) :: l) reached v st0 FUEL m LE' EVAL1) as RR;
@@ -745,23 +745,23 @@ Proof.
       destruct (eval C st1 e2 reached0 m) eqn:EVAL2'; eauto;
       try (
         specialize (HINT' H); destruct v; eauto; destruct st0;
-        assert (In cf (extract_reached (eval (C0 [|dy_c_lam x t ([||])|])
+        assert (In cf (extract_reached (eval (C0 [|dy_binde x t ([||])|])
                                            (ST (t !-> ev; mem) (tick C (ST mem t) x ev)) e
                                            reached1 m))) as HINT'';
         try (apply reach_myself; apply HINT');
-        destruct (eval (C0 [|dy_c_lam x t ([||])|])
+        destruct (eval (C0 [|dy_binde x t ([||])|])
                        (ST (t !-> ev; mem) (tick C (ST mem t) x ev)) e
                        reached1 m); eauto; destruct v; eauto);
       pose proof (relax_fuel C st1 e2 reached0 reached v st0 FUEL m LE' EVAL2) as RR';
       rewrite RR' in EVAL2'; inversion EVAL2'; subst.
       destruct v0; eauto. destruct st2.
-      specialize (IHFUEL (C0 [|dy_c_lam x t ([||])|])
+      specialize (IHFUEL (C0 [|dy_binde x t ([||])|])
                          (ST (t !-> ev; mem) (tick C (ST mem t) x ev)) e
                          reached1 m LE') as HINT''.
-      destruct (eval (C0 [|dy_c_lam x t ([||])|])
+      destruct (eval (C0 [|dy_binde x t ([||])|])
                      (ST (t !-> ev; mem) (tick C (ST mem t) x ev)) e
                      reached1 FUEL) eqn:EVAL3;
-      destruct (eval (C0 [|dy_c_lam x t ([||])|])
+      destruct (eval (C0 [|dy_binde x t ([||])|])
                      (ST (t !-> ev; mem) (tick C (ST mem t) x ev)) e
                      reached1 m) eqn:EVAL3'; eauto;
       try (destruct v; eauto); destruct v0; eauto.
@@ -787,29 +787,29 @@ Proof.
       destruct (eval C st e1 (Config C st (m_lete x e1 e2) :: l) m) eqn:EVAL1'; eauto;
       try (
         destruct v; eauto; destruct st0;
-        assert (In cf (extract_reached (eval (C [|dy_c_lete x t ([||])|])
+        assert (In cf (extract_reached (eval (C [|dy_binde x t ([||])|])
                                              (ST (t !-> ev; mem) (tick C (ST mem t) x ev)) e2
                                              reached0 m))) as HINT';
         try (apply reach_myself; apply HINT; eauto);
-        destruct (eval (C [|dy_c_lete x t ([||])|])
+        destruct (eval (C [|dy_binde x t ([||])|])
                        (ST (t !-> ev; mem) (tick C (ST mem t) x ev)) e2
                        reached0 m); eauto; destruct v; eauto; fail);
       pose proof (relax_fuel C st e1 (Config C st (m_lete x e1 e2) :: l) reached v st0 FUEL m LE' EVAL1) as RR;
       rewrite RR in EVAL1'; inversion EVAL1'; subst.
       destruct v0; eauto. destruct st1.
-      destruct (eval (C [|dy_c_lete x t ([||])|])
+      destruct (eval (C [|dy_binde x t ([||])|])
                      (ST (t !-> ev; mem) (tick C (ST mem t) x ev)) e2 reached0
                      FUEL) eqn:EVAL2; simpl;
-      destruct (eval (C [|dy_c_lete x t ([||])|])
+      destruct (eval (C [|dy_binde x t ([||])|])
                      (ST (t !-> ev; mem) (tick C (ST mem t) x ev)) e2 reached0
                      m) eqn:EVAL2';
       try (
-        assert (In cf (extract_reached (eval (C [|dy_c_lete x t ([||])|])
+        assert (In cf (extract_reached (eval (C [|dy_binde x t ([||])|])
                                              (ST (t !-> ev; mem) (tick C (ST mem t) x ev)) e2 reached0
                                              m))) as HINT';
         try (apply IHFUEL; eauto; rewrite EVAL2; eauto);
         rewrite EVAL2' in HINT'; eauto; destruct v; eauto);
-      pose proof (relax_fuel (C [|dy_c_lete x t ([||])|])
+      pose proof (relax_fuel (C [|dy_binde x t ([||])|])
                              (ST (t !-> ev; mem) (tick C (ST mem t) x ev)) e2
                              reached0 reached v st0 FUEL m LE' EVAL2) as RR';
       rewrite RR' in EVAL2'; inversion EVAL2'; subst.
@@ -819,19 +819,19 @@ Proof.
       destruct (eval C st e1 (Config C st (m_letm M e1 e2) :: l) m) eqn:EVAL1'; eauto;
       try (
         destruct v; eauto;
-        assert (In cf (extract_reached (eval (C [|dy_c_letm M mv ([||])|]) st0 e2 reached0 m))) as HINT';
+        assert (In cf (extract_reached (eval (C [|dy_bindm M mv ([||])|]) st0 e2 reached0 m))) as HINT';
         try (apply reach_myself; apply HINT; eauto);
-        destruct (eval (C [|dy_c_letm M mv ([||])|]) st0 e2 reached0 m); eauto; destruct v; eauto; fail);
+        destruct (eval (C [|dy_bindm M mv ([||])|]) st0 e2 reached0 m); eauto; destruct v; eauto; fail);
       pose proof (relax_fuel C st e1 (Config C st (m_letm M e1 e2) :: l) reached v st0 FUEL m LE' EVAL1) as RR;
       rewrite RR in EVAL1'; inversion EVAL1'; subst.
       destruct v0; eauto.
-      destruct (eval (C [|dy_c_letm M mv ([||])|]) st1 e2 reached0 FUEL) eqn:EVAL2; simpl;
-      destruct (eval (C [|dy_c_letm M mv ([||])|]) st1 e2 reached0 m) eqn:EVAL2';
+      destruct (eval (C [|dy_bindm M mv ([||])|]) st1 e2 reached0 FUEL) eqn:EVAL2; simpl;
+      destruct (eval (C [|dy_bindm M mv ([||])|]) st1 e2 reached0 m) eqn:EVAL2';
       try (
-        assert (In cf (extract_reached (eval (C [|dy_c_letm M mv ([||])|]) st1 e2 reached0 m))) as HINT';
+        assert (In cf (extract_reached (eval (C [|dy_bindm M mv ([||])|]) st1 e2 reached0 m))) as HINT';
         try (apply IHFUEL; eauto; rewrite EVAL2; eauto);
         rewrite EVAL2' in HINT'; eauto; destruct v; eauto; fail);
-      pose proof (relax_fuel (C [|dy_c_letm M mv ([||])|]) st1 e2 reached0 reached v st0 FUEL m LE' EVAL2) as RR';
+      pose proof (relax_fuel (C [|dy_bindm M mv ([||])|]) st1 e2 reached0 reached v st0 FUEL m LE' EVAL2) as RR';
       rewrite RR' in EVAL2'; inversion EVAL2'; subst.
       destruct v0; eauto.
 Qed.
@@ -872,14 +872,14 @@ Proof.
     try (assert False as contra; eauto; inversion contra); eauto.
     destruct IHr as [RR [RR' CONTAINED']]. rewrite <- RR in *. rewrite <- RR' in *. clear RR RR'.
     destruct v; eauto. destruct st2.
-    specialize (IHFUEL (C0 [|dy_c_lam x t ([||])|])
+    specialize (IHFUEL (C0 [|dy_binde x t ([||])|])
                        (ST (t !-> ev; mem) (tick C (ST mem t) x ev))
                        e reached1 reached2 CONTAINED').
     clear CONTAINED'.
-    destruct (eval (C0 [|dy_c_lam x t ([||])|])
+    destruct (eval (C0 [|dy_binde x t ([||])|])
                    (ST (t !-> ev; mem) (tick C (ST mem t) x ev))
                    e reached1 FUEL);
-    destruct (eval (C0 [|dy_c_lam x t ([||])|])
+    destruct (eval (C0 [|dy_binde x t ([||])|])
                    (ST (t !-> ev; mem) (tick C (ST mem t) x ev))
                    e reached2 FUEL);
     try (assert False as contra; eauto; inversion contra); eauto.
@@ -913,13 +913,13 @@ Proof.
     try (assert False as contra; eauto; inversion contra); eauto.
     destruct IHl as [RR [RR' CONTAINED']]. rewrite <- RR in *. rewrite <- RR' in *. clear RR RR'.
     destruct v; eauto. destruct st0.
-    specialize (IHFUEL (C [|dy_c_lete x t ([||])|])
+    specialize (IHFUEL (C [|dy_binde x t ([||])|])
                        (ST (t !-> ev; mem) (tick C (ST mem t) x ev))
                        e2 reached reached0 CONTAINED'). clear CONTAINED'.
-    destruct (eval (C [|dy_c_lete x t ([||])|])
+    destruct (eval (C [|dy_binde x t ([||])|])
                    (ST (t !-> ev; mem) (tick C (ST mem t) x ev))
                    e2 reached FUEL);
-    destruct (eval (C [|dy_c_lete x t ([||])|])
+    destruct (eval (C [|dy_binde x t ([||])|])
                    (ST (t !-> ev; mem) (tick C (ST mem t) x ev))
                    e2 reached0 FUEL);
     try (assert False as contra; eauto; inversion contra); eauto.
@@ -936,9 +936,9 @@ Proof.
     try (assert False as contra; eauto; inversion contra); eauto.
     destruct IHl as [RR [RR' CONTAINED']]. rewrite <- RR in *. rewrite <- RR' in *. clear RR RR'.
     destruct v; eauto.
-    specialize (IHFUEL (C [|dy_c_letm M mv ([||])|]) st0 e2 reached reached0 CONTAINED'). clear CONTAINED'.
-    destruct (eval (C [|dy_c_letm M mv ([||])|]) st0 e2 reached FUEL);
-    destruct (eval (C [|dy_c_letm M mv ([||])|]) st0 e2 reached0 FUEL);
+    specialize (IHFUEL (C [|dy_bindm M mv ([||])|]) st0 e2 reached reached0 CONTAINED'). clear CONTAINED'.
+    destruct (eval (C [|dy_bindm M mv ([||])|]) st0 e2 reached FUEL);
+    destruct (eval (C [|dy_bindm M mv ([||])|]) st0 e2 reached0 FUEL);
     try (assert False as contra; eauto; inversion contra); eauto.
     destruct IHFUEL as [RR [RR' CONTAINED']]. rewrite <- RR in *. rewrite <- RR' in *.
     destruct v; eauto.
@@ -988,19 +988,19 @@ Proof.
       try (rewrite HINT2 in H; rewrite HINT2'; rewrite HINT1 in H; rewrite HINT1';
           destruct H as [[[?|?]|?]|?]; simpl in *; eauto).
       destruct st2.
-      specialize (IHFUEL (C0 [|dy_c_lam x t ([||])|])
+      specialize (IHFUEL (C0 [|dy_binde x t ([||])|])
                          (ST (t !-> ev; mem) (tick C (ST mem t) x ev)) 
                          e reached1 cf) as HINT3.
-      specialize (IHFUEL (C0 [|dy_c_lam x t ([||])|])
+      specialize (IHFUEL (C0 [|dy_binde x t ([||])|])
                          (ST (t !-> ev; mem) (tick C (ST mem t) x ev)) 
                          e reached2 cf) as HINT3'.
-      pose proof (reach_same FUEL (C0 [|dy_c_lam x t ([||])|])
+      pose proof (reach_same FUEL (C0 [|dy_binde x t ([||])|])
                                   (ST (t !-> ev; mem) (tick C (ST mem t) x ev))
                                   e reached2 reached1 CONTAINED) as contra. clear CONTAINED.
-      destruct (eval (C0 [|dy_c_lam x t ([||])|])
+      destruct (eval (C0 [|dy_binde x t ([||])|])
                      (ST (t !-> ev; mem) (tick C (ST mem t) x ev)) e
                      reached1 FUEL);
-      destruct (eval (C0 [|dy_c_lam x t ([||])|])
+      destruct (eval (C0 [|dy_binde x t ([||])|])
                      (ST (t !-> ev; mem) (tick C (ST mem t) x ev)) e
                      reached2 FUEL);
       try (rewrite HINT3 in H); try rewrite HINT3';
@@ -1056,20 +1056,20 @@ Proof.
       destruct contra as [RR [RR' CONTAINED]]. rewrite RR in *. rewrite RR' in *. clear RR RR'.
       destruct v;
       try (rewrite HINT1 in H; rewrite HINT1'; destruct H as [[?|?]|?]; simpl in *; eauto). destruct st0.
-      specialize (IHFUEL (C [|dy_c_lete x t ([||])|])
+      specialize (IHFUEL (C [|dy_binde x t ([||])|])
                          (ST (t !-> ev; mem) (tick C (ST mem t) x ev))
                          e2 reached cf) as HINT2.
-      specialize (IHFUEL (C [|dy_c_lete x t ([||])|])
+      specialize (IHFUEL (C [|dy_binde x t ([||])|])
                          (ST (t !-> ev; mem) (tick C (ST mem t) x ev))
                          e2 reached0 cf) as HINT2'.
-      pose proof (reach_same FUEL (C [|dy_c_lete x t ([||])|])
+      pose proof (reach_same FUEL (C [|dy_binde x t ([||])|])
                                   (ST (t !-> ev; mem) (tick C (ST mem t) x ev))
                                   e2 reached0 reached CONTAINED) as contra.
       clear CONTAINED.
-      destruct (eval (C [|dy_c_lete x t ([||])|])
+      destruct (eval (C [|dy_binde x t ([||])|])
                      (ST (t !-> ev; mem) (tick C (ST mem t) x ev))
                      e2 reached FUEL);
-      destruct (eval (C [|dy_c_lete x t ([||])|])
+      destruct (eval (C [|dy_binde x t ([||])|])
                      (ST (t !-> ev; mem) (tick C (ST mem t) x ev))
                      e2 reached0 FUEL);
       try (rewrite HINT2 in H); try rewrite HINT2';
@@ -1095,12 +1095,12 @@ Proof.
       destruct contra as [RR [RR' CONTAINED]]. rewrite RR in *. rewrite RR' in *. clear RR RR'.
       destruct v;
       try (rewrite HINT1 in H; rewrite HINT1'; destruct H as [[?|?]|?]; simpl in *; eauto).
-      specialize (IHFUEL (C [|dy_c_letm M mv ([||])|]) st0 e2 reached cf) as HINT2.
-      specialize (IHFUEL (C [|dy_c_letm M mv ([||])|]) st0 e2 reached0 cf) as HINT2'.
-      pose proof (reach_same FUEL (C [|dy_c_letm M mv ([||])|]) st0 e2 reached0 reached CONTAINED) as contra.
+      specialize (IHFUEL (C [|dy_bindm M mv ([||])|]) st0 e2 reached cf) as HINT2.
+      specialize (IHFUEL (C [|dy_bindm M mv ([||])|]) st0 e2 reached0 cf) as HINT2'.
+      pose proof (reach_same FUEL (C [|dy_bindm M mv ([||])|]) st0 e2 reached0 reached CONTAINED) as contra.
       clear CONTAINED.
-      destruct (eval (C [|dy_c_letm M mv ([||])|]) st0 e2 reached FUEL);
-      destruct (eval (C [|dy_c_letm M mv ([||])|]) st0 e2 reached0 FUEL);
+      destruct (eval (C [|dy_bindm M mv ([||])|]) st0 e2 reached FUEL);
+      destruct (eval (C [|dy_bindm M mv ([||])|]) st0 e2 reached0 FUEL);
       try (rewrite HINT2 in H); try rewrite HINT2';
       try (rewrite HINT1 in H); try rewrite HINT1';
       try (simpl in *; destruct H as [[[?|?]|?]|?]; eauto; fail);
@@ -1143,19 +1143,19 @@ Proof.
       try (rewrite HINT2 in H; rewrite HINT2'; rewrite HINT1 in H; rewrite HINT1';
           destruct H as [?|[[[?|?]|?]|?]]; simpl in *; eauto; inversion H).
       destruct st2.
-      specialize (IHFUEL (C0 [|dy_c_lam x t ([||])|])
+      specialize (IHFUEL (C0 [|dy_binde x t ([||])|])
                          (ST (t !-> ev; mem) (tick C (ST mem t) x ev)) 
                          e reached1 cf) as HINT3'.
-      specialize (IHFUEL (C0 [|dy_c_lam x t ([||])|])
+      specialize (IHFUEL (C0 [|dy_binde x t ([||])|])
                          (ST (t !-> ev; mem) (tick C (ST mem t) x ev)) 
                          e reached2 cf) as HINT3.
-      pose proof (reach_same FUEL (C0 [|dy_c_lam x t ([||])|])
+      pose proof (reach_same FUEL (C0 [|dy_binde x t ([||])|])
                                   (ST (t !-> ev; mem) (tick C (ST mem t) x ev))
                                   e reached2 reached1 CONTAINED) as contra. clear CONTAINED.
-      destruct (eval (C0 [|dy_c_lam x t ([||])|])
+      destruct (eval (C0 [|dy_binde x t ([||])|])
                      (ST (t !-> ev; mem) (tick C (ST mem t) x ev)) e
                      reached1 FUEL);
-      destruct (eval (C0 [|dy_c_lam x t ([||])|])
+      destruct (eval (C0 [|dy_binde x t ([||])|])
                      (ST (t !-> ev; mem) (tick C (ST mem t) x ev)) e
                      reached2 FUEL);
       try (rewrite HINT3 in H); try rewrite HINT3';
@@ -1211,20 +1211,20 @@ Proof.
       destruct contra as [RR [RR' CONTAINED]]. rewrite RR in *. rewrite RR' in *. clear RR RR'.
       destruct v;
       try (rewrite HINT1 in H; rewrite HINT1'; destruct H as [?|[[?|?]|?]]; simpl in *; eauto; inversion H). destruct st0.
-      specialize (IHFUEL (C [|dy_c_lete x t ([||])|])
+      specialize (IHFUEL (C [|dy_binde x t ([||])|])
                          (ST (t !-> ev; mem) (tick C (ST mem t) x ev))
                          e2 reached cf) as HINT2'.
-      specialize (IHFUEL (C [|dy_c_lete x t ([||])|])
+      specialize (IHFUEL (C [|dy_binde x t ([||])|])
                          (ST (t !-> ev; mem) (tick C (ST mem t) x ev))
                          e2 reached0 cf) as HINT2.
-      pose proof (reach_same FUEL (C [|dy_c_lete x t ([||])|])
+      pose proof (reach_same FUEL (C [|dy_binde x t ([||])|])
                                   (ST (t !-> ev; mem) (tick C (ST mem t) x ev))
                                   e2 reached0 reached CONTAINED) as contra.
       clear CONTAINED.
-      destruct (eval (C [|dy_c_lete x t ([||])|])
+      destruct (eval (C [|dy_binde x t ([||])|])
                      (ST (t !-> ev; mem) (tick C (ST mem t) x ev))
                      e2 reached FUEL);
-      destruct (eval (C [|dy_c_lete x t ([||])|])
+      destruct (eval (C [|dy_binde x t ([||])|])
                      (ST (t !-> ev; mem) (tick C (ST mem t) x ev))
                      e2 reached0 FUEL);
       try (rewrite HINT2 in H); try rewrite HINT2';
@@ -1250,12 +1250,12 @@ Proof.
       destruct contra as [RR [RR' CONTAINED]]. rewrite RR in *. rewrite RR' in *. clear RR RR'.
       destruct v;
       try (rewrite HINT1 in H; rewrite HINT1'; destruct H as [?|[[?|?]|?]]; simpl in *; eauto; inversion H).
-      specialize (IHFUEL (C [|dy_c_letm M mv ([||])|]) st0 e2 reached cf) as HINT2'.
-      specialize (IHFUEL (C [|dy_c_letm M mv ([||])|]) st0 e2 reached0 cf) as HINT2.
-      pose proof (reach_same FUEL (C [|dy_c_letm M mv ([||])|]) st0 e2 reached0 reached CONTAINED) as contra.
+      specialize (IHFUEL (C [|dy_bindm M mv ([||])|]) st0 e2 reached cf) as HINT2'.
+      specialize (IHFUEL (C [|dy_bindm M mv ([||])|]) st0 e2 reached0 cf) as HINT2.
+      pose proof (reach_same FUEL (C [|dy_bindm M mv ([||])|]) st0 e2 reached0 reached CONTAINED) as contra.
       clear CONTAINED.
-      destruct (eval (C [|dy_c_letm M mv ([||])|]) st0 e2 reached FUEL);
-      destruct (eval (C [|dy_c_letm M mv ([||])|]) st0 e2 reached0 FUEL);
+      destruct (eval (C [|dy_bindm M mv ([||])|]) st0 e2 reached FUEL);
+      destruct (eval (C [|dy_bindm M mv ([||])|]) st0 e2 reached0 FUEL);
       try (rewrite HINT2 in H); try rewrite HINT2';
       try (rewrite HINT1 in H); try rewrite HINT1';
       try (simpl in *; destruct H as [?|[[[?|?]|?]|?]]; eauto; inversion H; fail);
@@ -1288,7 +1288,7 @@ Proof.
     assert (In (Config C' st' e') (extract_reached (Resolved v st1 reached0))).
     { rewrite <- EVAL2; rewrite separate_reach; eauto. }
     destruct v; simpl in *; eauto. destruct st1.
-    destruct (eval (C0 [|dy_c_lam x t ([||])|])
+    destruct (eval (C0 [|dy_binde x t ([||])|])
                    (ST (t !-> ev; mem) (tick C (ST mem t) x ev))
                    e reached0 FUEL) eqn:EVAL3;
     try (rewrite <- EVAL3; rewrite separate_reach; eauto).
@@ -1312,7 +1312,7 @@ Proof.
     { rewrite <- EVAL2; rewrite separate_reach.
       right. apply relax_fuel_reach with (FUEL := FUEL). nia. eauto. }
     destruct v0; simpl in *; eauto. destruct st1.
-    destruct (eval (C_lam [|dy_c_lam x t ([||])|])
+    destruct (eval (C_lam [|dy_binde x t ([||])|])
                    (ST (t !-> ev; mem) (tick C (ST mem t) x ev))
                    e reached0 (Nat.max FUEL FUEL')) eqn:EVAL3;
     try (rewrite <- EVAL3; rewrite separate_reach; eauto).
@@ -1339,7 +1339,7 @@ Proof.
     assert (eval C st_lam e2 reached (Nat.max FUEL (Nat.max FUEL' FUEL'')) = Resolved (EVal arg) (ST mem t) reached0) as RR.
     { apply relax_fuel with (FUEL := FUEL''). nia. eauto. }
     rewrite RR. clear RR.
-    destruct (eval (C_lam [|dy_c_lam x t ([||])|])
+    destruct (eval (C_lam [|dy_binde x t ([||])|])
                    (ST (t !-> arg; mem) (tick C (ST mem t) x arg))
                    e reached0 (Nat.max FUEL (Nat.max FUEL' FUEL''))) eqn:EVAL3;
     try (rewrite <- EVAL3; apply relax_fuel_reach with (FUEL := FUEL); try nia; eauto;
@@ -1377,7 +1377,7 @@ Proof.
     assert (In (Config C' st' e') (extract_reached (Resolved v st0 reached))).
     { rewrite <- EVAL1; rewrite separate_reach; eauto. }
     destruct v; simpl in *; eauto. destruct st0.
-    destruct (eval (C [|dy_c_lete x t ([||])|])
+    destruct (eval (C [|dy_binde x t ([||])|])
                    (ST (t !-> ev; mem) (tick C (ST mem t) x ev))
                    m reached FUEL) eqn:EVAL2;
     try (rewrite <- EVAL2; rewrite separate_reach; eauto).
@@ -1394,7 +1394,7 @@ Proof.
     assert (eval C st e [Config C st (m_lete x e m)] (Nat.max FUEL FUEL') = Resolved (EVal v) (ST mem t) reached) as RR.
     { apply relax_fuel with (FUEL := FUEL'). nia. eauto. }
     simpl. rewrite RR. clear RR.
-    destruct (eval (C [|dy_c_lete x t ([||])|])
+    destruct (eval (C [|dy_binde x t ([||])|])
                    (ST (t !-> v; mem) (tick C (ST mem t) x v))
                    m reached (Nat.max FUEL FUEL')) eqn:EVAL2;
     try (rewrite <- EVAL2; apply relax_fuel_reach with (FUEL := FUEL); try nia; eauto;
@@ -1410,7 +1410,7 @@ Proof.
     assert (In (Config C' st' e') (extract_reached (Resolved v st0 reached))).
     { rewrite <- EVAL1; rewrite separate_reach; eauto. }
     destruct v; simpl in *; eauto. destruct st0.
-    destruct (eval (C [|dy_c_letm M mv ([||])|]) (ST mem t) m2 reached FUEL) eqn:EVAL2;
+    destruct (eval (C [|dy_bindm M mv ([||])|]) (ST mem t) m2 reached FUEL) eqn:EVAL2;
     try (rewrite <- EVAL2; rewrite separate_reach; eauto).
     assert (In (Config C' st' e') (extract_reached (Resolved v st0 reached0))).
     { rewrite <- EVAL2; rewrite separate_reach; eauto. }
@@ -1425,7 +1425,7 @@ Proof.
     assert (eval C st m1 [Config C st (m_letm M m1 m2)] (Nat.max FUEL FUEL') = Resolved (MVal C_M) st_M reached) as RR.
     { apply relax_fuel with (FUEL := FUEL'). nia. eauto. }
     simpl. rewrite RR. clear RR.
-    destruct (eval (C [|dy_c_letm M C_M ([||])|]) st_M m2 reached (Nat.max FUEL FUEL')) eqn:EVAL2;
+    destruct (eval (C [|dy_bindm M C_M ([||])|]) st_M m2 reached (Nat.max FUEL FUEL')) eqn:EVAL2;
     try (rewrite <- EVAL2; apply relax_fuel_reach with (FUEL := FUEL); try nia; eauto;
          rewrite separate_reach; eauto).
     assert (In (Config C' st' e') (extract_reached (Resolved v0 st1 reached0))).
@@ -1476,7 +1476,7 @@ Proof.
       rewrite EVAL2 in H.
       assert (EvalR C st0 e2 (EVal ev) (ST mem t)) as ARG.
       eauto. clear H.
-      destruct (eval (C0 [|dy_c_lam x t ([||])|])
+      destruct (eval (C0 [|dy_binde x t ([||])|])
                      (ST (t !-> ev; mem) (tick C (ST mem t) x ev))
                      e reached0 FUEL) eqn:EVAL3;
       try (rewrite <- EVAL3 in R; eauto; rewrite separate_reach in R; simpl in *;
@@ -1525,7 +1525,7 @@ Proof.
       rewrite EVAL1 in H. 
       assert (EvalR C st e1 (EVal (Closure x0 e C0)) st0) as EVALx.
       eauto. clear H. destruct st0.
-      destruct (eval (C [|dy_c_lete x t ([||])|])
+      destruct (eval (C [|dy_binde x t ([||])|])
                      (ST (t !-> Closure x0 e C0; mem) (tick C (ST mem t) x (Closure x0 e C0)))
                      e2 reached FUEL) eqn:EVAL2;
       try (rewrite <- EVAL2 in R; eauto; rewrite separate_reach in R; simpl in *;
@@ -1551,7 +1551,7 @@ Proof.
       rewrite EVAL1 in H. 
       assert (EvalR C st e1 (MVal mv) st0) as EVALm.
       eauto. clear H.
-      destruct (eval (C [|dy_c_letm M mv ([||])|]) st0 e2 reached FUEL) eqn:EVAL2;
+      destruct (eval (C [|dy_bindm M mv ([||])|]) st0 e2 reached FUEL) eqn:EVAL2;
       try (rewrite <- EVAL2 in R; eauto; rewrite separate_reach in R; simpl in *;
            destruct R as [R|R]; eauto;
            replace reached with (extract_reached (Resolved (MVal mv) st0 reached)) in R by reflexivity;
@@ -1601,18 +1601,18 @@ Proof.
       destruct v; eauto. destruct ev.
       destruct (eval C st0 e2 reached FUEL) eqn:ARG; eauto.
       destruct v; eauto. destruct st1.
-      destruct (eval (C0 [|dy_c_lam x t ([||])|])
+      destruct (eval (C0 [|dy_binde x t ([||])|])
                      (ST (t !-> ev; mem) (tick C (ST mem t) x ev))
                      e reached0 FUEL) eqn:BODY; eauto.
       destruct v; eauto.
-      pose proof (reach_same FUEL (C0 [|dy_c_lam x t ([||])|])
+      pose proof (reach_same FUEL (C0 [|dy_binde x t ([||])|])
                                   (ST (t !-> ev; mem) (tick C (ST mem t) x ev))
                                   e [] reached0 (HINT _ reached0)) as R.
       rewrite BODY in R.
-      destruct (eval (C0 [|dy_c_lam x t ([||])|])
+      destruct (eval (C0 [|dy_binde x t ([||])|])
                      (ST (t !-> ev; mem) (tick C (ST mem t) x ev))
                      e [] FUEL) eqn:BODY'; try (inversion R; fail).
-      specialize (IHFUEL (C0 [|dy_c_lam x t ([||])|])
+      specialize (IHFUEL (C0 [|dy_binde x t ([||])|])
                          (ST (t !-> ev; mem) (tick C (ST mem t) x ev))
                          e). rewrite BODY' in IHFUEL.
       destruct R as [RR [RR' R]]. rewrite RR in *. rewrite RR' in *. clear RR RR'.
@@ -1633,17 +1633,17 @@ Proof.
       exists C. exists (m_var M). rewrite ACCESS. simpl in *; eauto.
     + destruct (eval C st e1 [Config C st (m_lete x e1 e2)] FUEL) eqn:EVALx; eauto.
       destruct v; eauto. destruct st0.
-      destruct (eval (C [|dy_c_lete x t ([||])|])
+      destruct (eval (C [|dy_binde x t ([||])|])
                      (ST (t !-> ev; mem) (tick C (ST mem t) x ev))
                      e2 reached FUEL) eqn:BODY; eauto.
-      pose proof (reach_same FUEL (C [|dy_c_lete x t ([||])|])
+      pose proof (reach_same FUEL (C [|dy_binde x t ([||])|])
                                   (ST (t !-> ev; mem) (tick C (ST mem t) x ev))
                                   e2 [] reached (HINT _ reached)) as R.
       rewrite BODY in R.
-      destruct (eval (C [|dy_c_lete x t ([||])|])
+      destruct (eval (C [|dy_binde x t ([||])|])
                      (ST (t !-> ev; mem) (tick C (ST mem t) x ev))
                      e2 []) eqn:BODY'; try (inversion R; fail).
-      specialize (IHFUEL (C [|dy_c_lete x t ([||])|])
+      specialize (IHFUEL (C [|dy_binde x t ([||])|])
                          (ST (t !-> ev; mem) (tick C (ST mem t) x ev))
                          e2). rewrite BODY' in IHFUEL.
       destruct R as [RR [RR' R]]. rewrite RR in *. rewrite RR' in *. clear RR RR'.
@@ -1651,11 +1651,11 @@ Proof.
       destruct v; eauto.
     + destruct (eval C st e1 [Config C st (m_letm M e1 e2)] FUEL) eqn:EVALM; eauto.
       destruct v; eauto.
-      destruct (eval (C [|dy_c_letm M mv ([||])|]) st0 e2 reached FUEL) eqn:BODY; eauto.
-      pose proof (reach_same FUEL (C [|dy_c_letm M mv ([||])|]) st0 e2 [] reached (HINT _ reached)) as R.
+      destruct (eval (C [|dy_bindm M mv ([||])|]) st0 e2 reached FUEL) eqn:BODY; eauto.
+      pose proof (reach_same FUEL (C [|dy_bindm M mv ([||])|]) st0 e2 [] reached (HINT _ reached)) as R.
       rewrite BODY in R.
-      destruct (eval (C [|dy_c_letm M mv ([||])|]) st0 e2 []) eqn:BODY'; try (inversion R; fail).
-      specialize (IHFUEL (C [|dy_c_letm M mv ([||])|]) st0 e2). rewrite BODY' in IHFUEL.
+      destruct (eval (C [|dy_bindm M mv ([||])|]) st0 e2 []) eqn:BODY'; try (inversion R; fail).
+      specialize (IHFUEL (C [|dy_bindm M mv ([||])|]) st0 e2). rewrite BODY' in IHFUEL.
       destruct R as [RR [RR' R]]. rewrite RR in *. rewrite RR' in *. clear RR RR'.
       destruct IHFUEL as [C' [e' [CONTAINED EVAL]]].
       destruct v; eauto.
